Reedy/Matching.v
@@ -93,16 +93,4 @@ Section MatchingObject.
       destruct f. simpl.
       apply (Ehapply_dep (Nsq _ _ _) tt).
   Qed.
-
-  Definition matching_obj_map `{InvCat} (X : C ⇒ Uˢ) (z : C) :
-    (X _o z) → matching_object X z.
-  Proof.
-    intros x. cbn.
-    exists (λ (a : z // C), X _a (rc_obj a) x).
-    apply functional_extensionality_dep. intros f.
-    destruct f as [s t f]. destruct f as [f cond]. simpl in *.
-    destruct f as [uu hom comm_tr]. simpl in *. simpl_ids_in_I comm_tr.
-    destruct t,s. unfold rc_obj. simpl in *. rewrite <- comm_tr.
-    rewrite F_compose. reflexivity.
-  Defined.
 End MatchingObject.
