Reedy/Reedy.v
@@ -1,0 +1,11 @@
+  Definition matching_obj_map `{InvCat} (X : C ⇒ Uˢ) (z : C) :
+    (X _o z) → matching_object X z.
+  Proof.
+    intros x. cbn.
+    exists (λ (a : z // C), X _a (rc_obj a) x).
+    apply functional_extensionality_dep. intros f.
+    destruct f as [s t f]. destruct f as [f cond]. simpl in *.
+    destruct f as [uu hom comm_tr]. simpl in *. simpl_ids_in_I comm_tr.
+    destruct t,s. unfold rc_obj. simpl in *. rewrite <- comm_tr.
+    rewrite F_compose. reflexivity.
+  Defined.
